define so_instruction behavior

EvmOpcodes.v
@@ -3,6 +3,12 @@ Sources:
 "small ad-hoc symbolic interpreter" - https://gist.github.com/pirapira/0946d151e038393078c3
 CompCert - https://github.com/AbsInt/CompCert/blob/master/x86/Asm.v
 *)
+Require Import Bool.
+Require Import List.
+Require Import Nat.
+Require Import EqNat.
+Require Import Arith.PeanoNat.
+
 
 Inductive op1 : Type :=
   | OP_ISZERO
@@ -94,46 +100,80 @@ Inductive instruction : Type :=
   | I_SUICIDE
 .
 
-Require Import Bool List Nat EqNat.
-
-Require Import Vector.
-Require Import Arith.PeanoNat.
-Require Import FSets.FMapWeakList.
-Module Import MapNat := FMapWeakList.Make Nat.
-
-Definition cell := nat.
-Definition memory := MapNat.t nat.
-Definition stack_t := list cell.
-
-Variable size : nat.
-Variable code : Vector.t instruction size.
 
 
-Definition apply_1_1 (f : cell -> cell) (s : stack_t) : option stack_t :=
+Definition word := nat.
+
+(** The stack is represented as a Coq [list word]
+    plus a proof that its lenth is smaller than 1024 *)
+Record stack_t: Type := mkstack {
+  stckval: list word; 
+  stcksize: length stckval < 1024
+}.
+
+Lemma stack_pop_le {T: Type}: forall (c : T) cs (H : length (c::cs) < 1024),
+  length cs < 1024.
+Proof.
+  intros.
+  apply Lt.lt_S_n in H.
+  apply Nat.lt_lt_succ_r.
+  assumption.
+Qed.
+
+Definition pop (s : stack_t) : option stack_t :=
   match s with
-    | c1::cs => Some ((f c1)::cs)
+    | mkstack (c::cs) p => Some (mkstack cs (stack_pop_le c cs p))
     | _ => None
   end.
 
-Definition apply_2_1 (f : cell -> cell -> cell) (s : stack_t) : option stack_t :=
+Ltac consume H := 
+  simpl;
+  intros;
+  repeat (assumption || apply Lt.lt_S_n in H; apply Nat.lt_lt_succ_r).
+
+Lemma stack_app_le1 {T: Type}: forall (c : T) cs f (H : length (c::cs) < 1024),
+  length ((f c)::cs) < 1024.
+Proof.
+  consume H.
+Qed.
+
+Lemma stack_app_le2 {T: Type}: forall (c1 c2 : T) cs f (H : length (c1::c2::cs) < 1024),
+  length ((f c1 c2)::cs) < 1024.
+Proof.
+  consume H.
+Qed.
+
+Lemma stack_app_le3 {T: Type}: forall (c1 c2 c3: T) cs f (H : length (c1::c2::c3::cs) < 1024),
+  length ((f c1 c2 c3)::cs) < 1024.
+Proof.
+  consume H.
+Qed.
+
+Definition apply_1_1 (f : word -> word) (s : stack_t) : option stack_t :=
   match s with
-    | c1::c2::cs => Some ((f c1 c2)::cs)
+    | mkstack (c1::cs) p => Some (mkstack ((f c1)::cs) (stack_app_le1 c1 cs f p))
     | _ => None
   end.
 
-Definition apply_3_1 (f : cell -> cell -> cell -> cell) (s : stack_t) : option stack_t :=
+Definition apply_2_1 (f : word -> word -> word) (s : stack_t) : option stack_t :=
   match s with
-    | c1::c2::c3::cs => Some ((f c1 c2 c3)::cs)
+    | mkstack (c1::c2::cs) p => Some (mkstack ((f c1 c2)::cs)  (stack_app_le2 c1 c2 cs f p))
     | _ => None
   end.
 
-Definition eval_op1 (op : op1) (c : cell) : cell :=
+Definition apply_3_1 (f : word -> word -> word -> word) (s : stack_t) : option stack_t :=
+  match s with
+    | mkstack (c1::c2::c3::cs) p => Some (mkstack ((f c1 c2 c3)::cs)  (stack_app_le3 c1 c2 c3 cs f p))
+    | _ => None
+  end.
+
+Definition eval_op1 (op : op1) (c : word) : word :=
   match op with
     | OP_ISZERO => if c then 0 else 1
     | OP_NOT => if c then 0 else 1
   end.
 
-Definition eval_op2 (op : op2) (c1 c2 : cell) : cell :=
+Definition eval_op2 (op : op2) (c1 c2 : word) : word :=
   match op with
     | OP_ADD => c1 + c2
     | OP_MUL => c1 * c2
@@ -156,10 +196,108 @@ Definition eval_op2 (op : op2) (c1 c2 : cell) : cell :=
     | OP_BYTE *)
   end.
 
-Definition eval_op3 (op : op3) (c1 c2 c3 : cell) : cell :=
+Definition eval_op3 (op : op3) (c1 c2 c3 : word) : word :=
   match op with
     | OP_ADDMOD => c1
     | OP_MULMOD => c1
+  end.
+Require Import PeanoNat.
+
+Require Import Arith.Compare_dec.
+
+
+Definition push (xs : list word) :=
+  if length xs <? 1024 then Some xs else None.
+
+Theorem coerce (xs : list word) : {1024 <= length xs}+{length xs < 1024}.
+Proof.
+  apply le_lt_dec.
+Defined.
+
+Definition coerce' (xs : list word) : 
+  {1024 <= length xs}
+  +{exists (p:(length xs < 1024)) e, e = mkstack xs p}.
+Proof.
+  pose (coerce xs).
+  inversion s. 
+  - left. assumption.
+  - right. exists H. exists ({| stckval := xs; stcksize := H |}).
+    reflexivity.
+Defined.
+
+Lemma ltb_lt' {T: Type} : forall (e: T) n,
+  (if n <? 1024 then Some e else None) = Some e -> n < 1024.
+Proof.
+  intros.
+  pose (Nat.ltb_lt n 1024).
+  inversion i; apply H0; clear i.
+  destruct (n <? 1024). reflexivity. inversion H.
+Qed.
+
+Lemma p1 : forall xs, (exists xs', push xs = Some xs') <-> length xs < 1024.
+Proof.
+  intros. unfold push.
+  split.
+  - intro. apply (ltb_lt' xs).
+    destruct (length xs <? 1024) eqn:Q. reflexivity. inversion H as [H1 H2]. inversion H2.
+  - intros.
+    exists xs.
+
+      pose (Nat.ltb_lt (length xs) 1024). inversion i. clear i.
+    destruct (length xs <? 1024). reflexivity. apply H1 in H. inversion H.
+Qed.
+
+Lemma p2 : forall xs st, push xs = Some st -> length st < 1024.
+Proof.
+  unfold push.
+  intros.
+  apply (ltb_lt' xs).
+  destruct (length xs <? 1024) eqn:Q.
+  - inversion H. rewrite -> H1 in *.
+    rewrite -> Q. reflexivity.
+  - inversion H.
+Qed.
+
+Lemma firstn_lt_1024 {T: Type}: forall (l: list T), length (firstn 1023 l) < 1024.
+Proof.
+  intros.
+  apply Lt.le_lt_n_Sm.
+  rewrite -> firstn_length.
+  apply (Nat.le_min_l 1023 (length l)).
+Qed.
+
+Lemma qqq {T: Type}:
+  forall (l: list T), length l <? 1024 = true -> length l < 1024.
+Proof.
+  intros.
+  apply (Nat.ltb_lt (length l) 1024), H.
+Qed.
+
+
+Definition act (i : so_instruction) (s s' : stack_t) : Prop :=
+  match i, stckval s, stckval s' with
+   | I_STOP, _, _ => False
+   | I_POP   , (_::cs)         , st' => st' = cs
+   | I_POP   , _               , _   => False
+   | I_OP1 op, (c1::cs)        , st' => st' = (eval_op1 op c1)::cs
+   | I_OP1 _ , _               , _   => False
+   | I_OP2 op, (c1::c2::cs)    , st' => st' = (eval_op2 op c1 c2)::cs
+   | I_OP2 _ , _               , _   => False
+   | I_OP3 op, (c1::c2::c3::cs), st' => st' = (eval_op3 op c1 c2 c3)::cs
+   | I_OP3 _ , _               , _   => False
+   | I_PUSH (x::xs), st, st' => st' = (x::xs) ++ st
+   | I_PUSH _      , _ , _   => False
+   | I_DUP (S n), st, (c0::st') =>
+       st' = st
+       /\ List.nth_error st (S n) = Some c0
+   | I_DUP _, _, _ => False
+   | I_SWAP (S n), (c::cs), (c'::cs') =>
+       length (c::cs) > n
+       /\ skipn n cs = skipn n cs'
+       /\ firstn (n-1) cs = firstn (n-1) cs'
+       /\ List.nth_error cs  n = Some c'
+       /\ List.nth_error cs' n = Some c
+   | I_SWAP _, _, _ => False
   end.
 
 Definition exec_so_instr (i : so_instruction) (s : stack_t) : option stack_t :=
@@ -168,12 +306,18 @@ Definition exec_so_instr (i : so_instruction) (s : stack_t) : option stack_t :=
     | I_OP1 op => apply_1_1 (eval_op1 op) s
     | I_OP2 op => apply_2_1 (eval_op2 op) s
     | I_OP3 op => apply_3_1 (eval_op3 op) s
-    | I_POP => if s then Some (List.tl s) else None
-    | I_PUSH xs => if ltb (length (xs ++ s)) 1024 then Some (xs ++ s) else None
-    | I_DUP n => match List.nth_error s n with
+    | I_POP => pop s
+    | I_PUSH xs => let st' := xs ++ stckval s in
+                   match Reflect length st' <? 1024 with
+                     | ReflectT _ _ => Some (mkstack st' (qqq st'))
+                     | false => None
+                   end
+    | _ => None
+  end.
+    | I_DUP n => match List.nth_error (stckval s) n with
+                   | Some v => Some (mkstack (v::(stckval s)) (firstn_lt_1024 st'))
                    | None => None
-                   | Some v => Some (v::s)
-                  end
+                 end
     | I_SWAP n => let depth := firstn n s in
                   if ltb (length depth) n then None else Some (depth ++ s)
   end.
@@ -192,10 +336,21 @@ Definition exec_jump_instr (i : instruction) (pc : nat) (s : stack_t) : option n
     | _ => Some (pc + 1)
   end.
 
+Require Import Vector.
+Require Import FSets.FMapWeakList.
+Module Import MapNat := FMapWeakList.Make Nat.
+Definition byte := nat.
+Definition memory := MapNat.t byte.
+Definition storage := MapNat.t word.
+Variable size : nat.
+Variable code : Vector.t instruction size.
+
+
+
 
 Record state := State {
   stack : stack_t;
   mem  : memory;
-  pers : memory;
+  stor : storage;
   pc : nat;
 }.
