Uint256.v
@@ -1,0 +1,4 @@
+Require Import Coqlib.
+Require Import Words.
+
+Definition zlt := Z.ltb.
